Sorted out the source code (now it compiles!)
Out-commented a lot of the heap stuff (I think some libraries are
missing).

src/Hoare.v
@@ -1,12 +1,12 @@
 Require Export imp.
 Require Import FunctionalExtensionality.
 
-Definition Assertion := option exn -> state -> heap -> Prop.
+Definition Assertion := option exn -> state -> Prop.
 
 Definition assert_implies (P Q : Assertion) : Prop :=
   forall ex st, P ex st -> Q ex st.
 
-Definition safe c st h := ~ (ceval c st h empty_state h). 
+(*Definition safe c st h := ~ (ceval c st h empty_state h).*)
 
 Notation "P ->> Q" :=
   (assert_implies P Q) (at level 80) : hoare_spec_scope.
@@ -15,14 +15,22 @@ Open Scope hoare_spec_scope.
 Notation "P <<->> Q" :=
   (P ->> Q /\ Q ->> P) (at level 80) : hoare_spec_scope.
   
-Definition hoare_triple
+(*Definition hoare_triple
            (P:Assertion) (c:com) (Q:Assertion) : program -> Prop :=
   fun env =>
     forall st st' ex,
          safe c st h /\ forall st' h', ceval c env st h st' h' ex ->
          P None st h->
-         Q ex st' h'.
-  
+         Q ex st' h'.*)
+
+Definition hoare_triple
+           (P:Assertion) (c:com) (Q:Assertion) : program -> Prop :=
+  fun env =>
+    forall st st' ex,
+         ceval c env st st' ex ->
+         P None st ->
+         Q ex st'.
+
 Notation "{{ P }}  c  {{ Q }}" :=
   (hoare_triple P c Q) (at level 90, c at next level)
   : hoare_spec_scope.
@@ -287,8 +295,8 @@ Proof.
   assumption.
 Qed.
 
-Theorem hoare_alloc : forall x,
-  {{ emp }} x <-# ALLOC {{ x |-> ANum 0 }}.
+(*Theorem hoare_alloc : forall x,
+  {{ emp }} x <-# ALLOC {{ (x |-> ANum 0) }}.
 Proof.
   split.
   unfold safe.
@@ -445,190 +453,4 @@ Proof.
   admit.
   apply empty_map.
   apply H4.
-Qed.
-
-(*******************
- * EXAMPLE 1       *
- *******************)
-
-Definition body : com := 
-  Y ::= APlus (AId X) (ANum 1).
-  
-Definition env : program :=
-  fun id =>
-    if eq_funid_dec F id
-    then (body, [X], (APlus (AId X) (ANum 1)))
-    else (CSkip, [], ANum 0)
-    .
-
-Lemma body_p : forall X Y,
-  {{ (fun e st => st Y = st X + 1)[Y |-> (APlus (AId X) (ANum 1))] }}
-    Y ::= APlus (AId X) (ANum 1)
-  {{ (fun e st => st Y = st X + 1) }} env.
-Proof.
-  intros X Y.
-  apply hoare_consequence_post with (Q' := fun e st => st Y = st X + 1 /\ e = None).
-  eapply hoare_asgn.
-  intro; intros.
-  destruct H; assumption.
-Qed.
-
-(* Theorem prog_correct :
-  {{fun e st => True}}
-    CCall F Z [ANum 2]
-  {{fun e st => st Z = 3}} env.
-Proof.
-  eapply hoare_consequence_pre.
-  apply hoare_call with (params := [X]) (Q := fun e st => st Y = st X + 1)
-                  (body := body) (rexp := (APlus (AId X) (ANum 1)))
-                  (P := fun e st => st X = 2).
-  unfold env. simpl. reflexivity.
-  eapply hoare_consequence_pre.
-  apply hoare_consequence_post with (Q' := fun e st => st Y = st X + 1).
-  eapply body_p.
-  intro; intros.
-  simpl.
-  apply hoare_consequence_post
-  	with (Q' := fun e st => st Y = 3 /\ 3 = aeval st (APlus (AId X) (ANum 1)) /\ e = None).
-  apply hoare_asgn.
-  intro. intros _.
-  unfold assn_sub.
-  simpl.
-  split; try rewrite update_retrieve; reflexivity.
-Qed.
-
-( *******************
- * EXAMPLE 2       *
- ******************* )
-
-Definition Fbody : com := 
-  IFB (BEq (ANum 0) (AId X))
-  THEN Z ::= APlus (AId Y) (ANum 1)
-  ELSE CCall G Z [AId Y]
-  FI.
-  
-Definition Gbody : com := 
-  Z ::= APlus (AId Y) (ANum 1) ;;
-  Z ::= APlus (AId Z) (ANum 1)
-  .
-  
-Definition env'' : program :=
-  fun id =>
-    if eq_id_dec F id
-    then (Fbody, cons X (cons Y nil), (APlus (AId X) (AId Y)))
-    else if eq_id_dec G id
-    then (Gbody, [X], (APlus (AId X) (ANum 2)))
-    else (CSkip, [], ANum 0)  
-  .
-  
-Theorem prog_correct'' :
-  {{fun st => True}}
-    CCall F Z (cons (ANum 10) (cons (ANum 10) nil))
-  {{fun st => st Z = 20}} env''.
-Proof.
-  eapply hoare_consequence_pre.
-  apply hoare_call with (params := cons X (cons Y nil))
-			      (Q := fun st => st Z = st X + st Y)
-                  (body := Fbody) (rexp := (APlus (AId X) (AId Y)))
-                  (P := fun st => st X + st Y = st X + st Y /\ st X = 10 /\ st Y = 10).
-  unfold env''. simpl. reflexivity.
-  eapply hoare_consequence_post with (Q' := fun st => st Z = st X + st Y /\ st X = 10 /\ st Y = 10).
-  eapply hoare_consequence_pre with (P' := fun st => True).
-  unfold body''.
-  apply b''.
-  intro; intros; apply I.
-  intro; intros.
-  destruct H.
-  split. assumption.
-  unfold aeval. destruct H0; rewrite H0, H1; reflexivity.
-  intros st _. simpl.
-  split. reflexivity.
-  rewrite update_retrieve_dif, update_retrieve, update_retrieve.
-  split; reflexivity.
-  unfold Y, X, not; intro; congruence.
-Qed. *)
-
-Definition body'' : com := 
-  IFB (BEq (ANum 1) (AId X))
-  THEN Z ::= APlus (AId Y) (AId X)
-  ELSE CCall F Z (cons (AMinus (AId X) (ANum 1))
-				   (cons (APlus (AId Y) (ANum 1))
- 					 nil))
-  FI.
-(*  
-Definition env'' : program :=
-  fun id =>
-    if eq_id_dec F id
-    then (body'', cons X (cons Y nil), (APlus (AId X) (AId Y)))
-    else (CSkip, [], ANum 0)
-    .
-
-( * 
-  {{ fun st => st X > 0 }} env
-  IFB (BEq (ANum 1) (AId X)) THEN
-    {{ fun st => st X = 1 /\ st X + Y = st X + Y }} env ->>
-    {{ fun st => st X + Y = st X + Y }} env
-    Z ::= APlus (AId X) (AId Y)
-    {{ fun st => st Z = st X + Y }} env
-  ELSE
-    {{ fun st => st X > 1 /\ st X + st Y = st X + st Y }} env
-    CCall F Z (cons (AMinus (AId X) (ANum 1))
-		   		 (cons (APlus (AId Y) (ANum 1))
- 					nil))
- 	{{ fun st => st X > 1 /\ st Z = st X + st Y }} env ->>
- 	{{ fun st => st Z = st X + st Y }} env
-  FI.
-  {{ fun st => st Z = st X + st Y }} env * )
-
-Lemma b'' : forall X Y Z x y z env,
-  z = x + y ->
-  {{ (fun st => z = st Z /\ x = st X /\ y = st Y)[Z |-> APlus (AId Y) (AId X)] }}
-  IFB (BEq (ANum 1) (AId X))
-  THEN Z ::= APlus (AId Y) (AId X)
-  ELSE CCall F Z (cons (AMinus (AId X) (ANum 1))
-				   (cons (APlus (AId Y) (ANum 1))
- 					 nil))
-  FI
-  {{ fun st => st Z = st X + st Y }} env.
-Proof.
-  intros X Y Z x y z env H.
-  apply hoare_if.
-  eapply hoare_consequence_post
-	with (Q' := fun st : state => st Z = st X + st Y).
-  eapply hoare_consequence_pre.
-  eapply hoare_asgn.
-  intro. intros.
-  unfold assn_sub in *.
-  destruct H0; destruct H0; destruct H2.
-  rewrite <- H0; rewrite <- H2; rewrite <- H3.
-  assumption.
-  intro; intros.
-  assumption.
-Admitted.
-
-Theorem prog_correct'' :
-  {{fun st => True}}
-    CCall F Z (cons (ANum 10) (cons (ANum 10) nil))
-  {{fun st => st Z = 20}} env''.
-Proof.
-  eapply hoare_consequence_pre.
-  apply call with (params := cons X (cons Y nil))
-			      (Q := fun st => st Z = st X + st Y)
-                  (body := body'') (rexp := (APlus (AId X) (AId Y)))
-                  (P := fun st => st X + st Y = st X + st Y /\ st X = 10 /\ st Y = 10).
-  unfold env''. simpl. reflexivity.
-  eapply hoare_consequence_post with (Q' := fun st => st Z = st X + st Y /\ st X = 10 /\ st Y = 10).
-  eapply hoare_consequence_pre with (P' := fun st => True).
-  unfold body''.
-  apply b''.
-  intro; intros; apply I.
-  intro; intros.
-  destruct H.
-  split. assumption.
-  unfold aeval. destruct H0; rewrite H0, H1; reflexivity.
-  intros st _. simpl.
-  split. reflexivity.
-  rewrite update_retrieve_dif, update_retrieve, update_retrieve.
-  split; reflexivity.
-  unfold Y, X, not; intro; congruence.
-Qed. *)
+Qed.*)
