src/imp_ast.v
@@ -69,7 +69,7 @@ Inductive com : Type :=
   | CWhile : bexp -> com -> com
   | CThrow : exid -> list aexp -> com
   | CTry : com -> exid -> list id -> com -> com
-  | CCall : funid -> id -> list aexp -> com.
+  | CCall : funid -> id -> list aexp -> com
   | CAlloc : id ->com
   | CRead : id -> aexp -> com
   | CWrite : aexp -> aexp -> com
